@prefix schema: <http://schema.org/> .
@prefix adms: <http://www.w3.org/ns/adms#> .
@prefix owl: <http://www.w3.org/2002/07/owl#> .
@prefix org: <http://www.w3.org/ns/org#> .
@prefix xsd: <http://www.w3.org/2001/XMLSchema#> .
@prefix skosthes: <http://purl.org/iso25964/skos-thes#> .
@prefix rdfs: <http://www.w3.org/2000/01/rdf-schema#> .
@prefix qb: <http://purl.org/linked-data/cube#> .
@prefix dct: <http://purl.org/dc/terms/> .
@prefix MomCare: <http://PharmAccess/MomCare/#> .
@prefix rdf: <http://www.w3.org/1999/02/22-rdf-syntax-ns#> .
@prefix doap: <http://usefulinc.com/ns/doap#> .
@prefix sh: <http://www.w3.org/ns/shacl#> .
@prefix dcat: <http://www.w3.org/ns/dcat#> .
@prefix euvoc: <http://publications.europa.eu/ontology/euvoc#> .
@prefix prov: <http://www.w3.org/ns/prov#> .
@prefix foaf: <http://xmlns.com/foaf/0.1/> .
@prefix dc: <http://purl.org/dc/elements/1.1/> .
@prefix skos: <http://www.w3.org/2004/02/skos/core#> .
@prefix skosxl: <http://www.w3.org/2008/05/skos-xl#> .

<http://PharmAccess/MomCare/> a skos:ConceptScheme;
  dct:title "MomCare vocabulary";
  dct:description "Vocabulary for data related to the PharmAccess MomCare program";
  dct:creator "fheddema";
  <pav:createdOn> "16-05-2023";
  skos:hasTopConcept MomCare:patient_overviews, MomCare:Beneficiary_id_careanalytics,
    MomCare:beneficiary_id, MomCare:Country, MomCare:Date_of_birth, MomCare:Age_at_enrolment,
    MomCare:Cohort, MomCare:Is_adult, MomCare:Age_group, MomCare:Enrolment_region, MomCare:Enrolment_date,
    MomCare:program_id, MomCare:Enrolment_provider_id, MomCare:Enrolment_provider_name,
    MomCare:Enrolment_week, MomCare:Risk_level, MomCare:Enrolment_trimester, MomCare:Week_risk_detection,
    MomCare:Risk_factors, MomCare:Current_week, MomCare:Expected_delivery_date, MomCare:Actual_delivery_date,
    MomCare:Delivery_type, MomCare:Date_finished, MomCare:Ancs, MomCare:Delivery, MomCare:Pncs,
    MomCare:Imms, MomCare:Delivery_out, MomCare:Diagnoses, MomCare:Total_costs, MomCare:Total_costs_eur,
    MomCare:Journey_score, MomCare:Dbt_recency_value, MomCare:Dwh_inserttime, MomCare:enrolment_survey,
    MomCare:Pregnancy_age_first_time, MomCare:Ability_read_write, MomCare:Clinic_visit_current_pregnancy_before,
    MomCare:Clinic_visit_previous_pregnancy, MomCare:Complications_previous_pregnancy,
    MomCare:Existing_health_conditions, MomCare:Household_television, MomCare:Household_electricity,
    MomCare:Pregnancy_history, MomCare:Travel_time, MomCare:Pregnancy_children_birth_number,
    MomCare:Household_persons, MomCare:Social_support_persons, MomCare:Household_rooms,
    MomCare:Pregnancy_history_amount_before, MomCare:Pregnancy_history_amount, MomCare:Household_hunger_pastyear,
    MomCare:Mental_experience_depression, MomCare:Mental_experience_interest, MomCare:Survey_language_choice,
    MomCare:Household_airtime_spendperweek, MomCare:Existing_health_conditions_other,
    MomCare:Pregnancy_EDD, MomCare:Household_educationlevel_head, MomCare:Household_material_walls,
    MomCare:Household_material_floor, MomCare:Household_material_roof, MomCare:Household_fuel_cooking,
    MomCare:Household_toilet_type, MomCare:Travel_means, MomCare:Clinic_referral_source,
    MomCare:Household_radio, MomCare:Household_iron, MomCare:Household_bankaccount, MomCare:Household_source_energy,
    MomCare:Height, MomCare:Obstetric_history, MomCare:Lifestyle_smokedrinkdrugs, MomCare:sms_survey,
    MomCare:Household_chronic_condition, MomCare:Breastfeeding_yesno, MomCare:Improve_services,
    MomCare:Improve_comfort, MomCare:Breastfeeding_confidence, MomCare:Breastfeeding_confidence_spaces,
    MomCare:Household_adults, MomCare:Household_children, MomCare:Role_preparation, MomCare:Role_preparation_spaces,
    MomCare:Experience_lamazeclass, MomCare:Social_satisfaction, MomCare:Quality_of_life,
    MomCare:Quality_of_life_spaces, MomCare:Residence_county, MomCare:Improve_experience_like_dislike_postnatal,
    MomCare:Information_next_visit, MomCare:Breastfeeding_support_received, MomCare:Improve_service_clinic,
    MomCare:Improve_service_clinic_2, MomCare:Improve_experience_like_dislike, MomCare:Improve_experience_like_dislike_2,
    MomCare:Improve_experience_like_dislike_registration, MomCare:Service_satisfaction,
    MomCare:Service_comfort, MomCare:Improve_experience_like_dislike_delivery, MomCare:Delivery_respect,
    MomCare:Delivery_wellhandled, MomCare:Breastfeeding_currentmode, MomCare:Breastfeeding_preference,
    MomCare:Delivery_out_where, MomCare:Service_satisfaction_secondclinic, MomCare:Improve_experience_how,
    MomCare:Role_feelings, MomCare:Service_like_1, MomCare:Recommend_to_others, MomCare:Service_payment,
    MomCare:Service_satisfaction_1, MomCare:Breastfeeding_mode, MomCare:Service_payment_what,
    MomCare:Feedback_consent_1, MomCare:Breastfeeding_time, MomCare:Feedback_consent,
    MomCare:Service_satisfaction_2, MomCare:Care_usage_tests, MomCare:Service_like_2,
    MomCare:Service_dislike, MomCare:Care_usage_tests_other, MomCare:Care_usage_services,
    MomCare:Service_satisfaction_3, MomCare:Improve_how, MomCare:Improve_why, MomCare:Satisfaction_why_not,
    MomCare:eoj_call, MomCare:StartingDate, MomCare:EndingDate, MomCare:InterviewerID,
    MomCare:contactid, MomCare:Consent_participation, MomCare:Education_level, MomCare:Child_alive,
    MomCare:Child_age, MomCare:Child_age_text, MomCare:Interview_continue, MomCare:Child_age_of_death,
    MomCare:Child_age_of_death_text, MomCare:Child_cause_of_death, MomCare:Child_cause_of_death_text,
    MomCare:Clinic_visit_outside_1, MomCare:Clinic_visit_outside_n, MomCare:Clinic_visit_outside_reason,
    MomCare:Clinic_visit_outside_reason_text, MomCare:Hospital_name, MomCare:Facility_type_hospital,
    MomCare:Transport_mode_facility, MomCare:Facility_type_delivery, MomCare:Facility_name_delivery,
    MomCare:Delivery_weeks_along, MomCare:Delivery_complications_1, MomCare:Information_pregnancy,
    MomCare:ANC_booklet, MomCare:Inform_time_delivery_visit, MomCare:Transport_mode_delivery,
    MomCare:Facility_delivery_choice_reason, MomCare:Facility_delivery_choice_reason_text,
    MomCare:Recommend_facility_delivery, MomCare:Recommend_facility_delivery_text, MomCare:Delivery_rating,
    MomCare:Delivery_danger_signs, MomCare:Information_enough, MomCare:Support_delivery,
    MomCare:Support_ANC_PNC, MomCare:Breastfeeding_information, MomCare:Breastfeeding_challenges_1,
    MomCare:Breastfeeding_challenges_text, MomCare:Health_challenges_daily_1, MomCare:Mental_experience_post_delivery_1,
    MomCare:Counselling, MomCare:Experience_overall, MomCare:Experience_overall_reason,
    MomCare:tz-diagn, MomCare:PATIENT_ID, MomCare:DATE_OF_BIRTH, MomCare:AGE_AT_ENROLMENT,
    MomCare:ENROLMENT_DATE, MomCare:ENROLMENT_PROVIDER_ID, MomCare:ENROLMENT_PROVIDER_NAME,
    MomCare:ENROLMENT_PROVIDER_LEVEL, MomCare:ENROLMENT_REGION, MomCare:VISIT_ID, MomCare:VISIT_DATE,
    MomCare:VISIT_NUMBER, MomCare:VISIT_TYPE, MomCare:VISIT_PROVIDER_ID, MomCare:VISIT_PROVIDER_NAME,
    MomCare:VISIT_PROVIDER_LEVEL, MomCare:VISIT_PROVIDER_REGION, MomCare:EVENT, MomCare:EVENT_ID,
    MomCare:EVENT_DESCRIPTION, MomCare:DIAGN_DESCRIPTION, MomCare:DIAGN_CODE, MomCare:EVENT_COSTS,
    MomCare:VISIT_DIAGN_NO, MomCare:DIAGN_NO, MomCare:ke-diagn, MomCare:EVENT_TYPE, MomCare:TREATMENT_ID,
    MomCare:REFERENCE, MomCare:DATE_TREATMENT, MomCare:PROVIDER_ID, MomCare:PROVIDER,
    MomCare:TREATMENT_STATUS, MomCare:PAYMENT_STATUS, MomCare:TOTAL_COST, MomCare:VISIT_DIAGNOSIS_ID,
    MomCare:DIAGNOSIS_ID, MomCare:DIAGN_LABEL, MomCare:DIAGN_CAT, MomCare:DIAG_gen, MomCare:DIAGNOSIS,
    MomCare:DIAGNOSIS_CA, MomCare:VISIT_NO, MomCare:ke-items, MomCare:CARE_ANALYTICS_ID,
    MomCare:BENEFICIARY_ID_ORG, MomCare:ITEM_ID, MomCare:ITEM_CODE, MomCare:ITEM_NAME,
    MomCare:tz-items, MomCare:VISIT_ITEM_NO, MomCare:ITEM_NO, MomCare:safe_care, <http://PharmAccess/MomCare/#Assessment%20ID>,
    <http://PharmAccess/MomCare/#Facility%20ID>, MomCare:Facility, MomCare:District, MomCare:Region,
    <http://PharmAccess/MomCare/#Facility%20category>, MomCare:Latitude, MomCare:Longitude,
    <http://PharmAccess/MomCare/#Approval%20date>, <http://PharmAccess/MomCare/#Visit%20number>,
    <http://PharmAccess/MomCare/#Type%20of%20ownership>, MomCare:Location, <http://PharmAccess/MomCare/#Assessment%20Tool>,
    MomCare:Version, <http://PharmAccess/MomCare/#Team%20leader>, <http://PharmAccess/MomCare/#Team%20members>,
    <http://PharmAccess/MomCare/#First%20reviewer>, <http://PharmAccess/MomCare/#SC%20Level%20calculated>,
    <http://PharmAccess/MomCare/#SafeCare%20Score%20Rating%20(Basic)>, <http://PharmAccess/MomCare/#SafeCare%20Score%20Advanced>,
    <http://PharmAccess/MomCare/#SC%20Level%20awarded>, MomCare:Organization, MomCare:Program,
    <http://PharmAccess/MomCare/#SE1%20Score>, <http://PharmAccess/MomCare/#SE2%20Score>,
    <http://PharmAccess/MomCare/#SE3%20Score>, <http://PharmAccess/MomCare/#SE4%20Score>,
    <http://PharmAccess/MomCare/#SE5%20Score>, <http://PharmAccess/MomCare/#SE6%20Score>,
    <http://PharmAccess/MomCare/#SE7%20Score>, <http://PharmAccess/MomCare/#SE8%20Score>,
    <http://PharmAccess/MomCare/#SE9%20Score>, <http://PharmAccess/MomCare/#SE10%20Score>,
    <http://PharmAccess/MomCare/#SE11%20Score>, <http://PharmAccess/MomCare/#SE12%20Score>,
    <http://PharmAccess/MomCare/#SE13%20Score> .

MomCare:patient_overviews a skos:Concept;
  skos:prefLabel "patient_overviews"@en;
  skos:definition "This is a set of controlled terms for the Patient Overviews.";
  skos:inScheme <http://PharmAccess/MomCare/>;
  skos:topConceptOf <http://PharmAccess/MomCare/> .

MomCare:Beneficiary_id_careanalytics a skos:Concept;
  skos:prefLabel "Beneficiary_id_careanalytics"@en;
  skos:definition "Identifier for those enrolled in the MomCare program and registered in Care Analytics (only Kenyan beneficiaries).";
  skos:inScheme <http://PharmAccess/MomCare/>;
  skos:topConceptOf <http://PharmAccess/MomCare/> .

MomCare:beneficiary_id a skos:Concept;
  skos:prefLabel "beneficiary_id"@en;
  skos:definition "Identifier for all those enrolled in the MomCare program.";
  skos:inScheme <http://PharmAccess/MomCare/>;
  skos:topConceptOf <http://PharmAccess/MomCare/> .

MomCare:Country a skos:Concept;
  skos:prefLabel "Country"@en;
  skos:definition "Nation of enrolment in MomCare program.", "Country location of care provider as registered by SafeCare.";
  skos:inScheme <http://PharmAccess/MomCare/>;
  skos:topConceptOf <http://PharmAccess/MomCare/> .

MomCare:Date_of_birth a skos:Concept;
  skos:prefLabel "Date_of_birth"@en;
  skos:definition "Date of birth of identified beneficiary.", "Date of Birth";
  skos:inScheme <http://PharmAccess/MomCare/>;
  skos:topConceptOf <http://PharmAccess/MomCare/> .

MomCare:Age_at_enrolment a skos:Concept;
  skos:prefLabel "Age_at_enrolment"@en;
  skos:definition "Age at enrolment derived from date of birth and enrolment date.";
  skos:inScheme <http://PharmAccess/MomCare/>;
  skos:topConceptOf <http://PharmAccess/MomCare/> .

MomCare:Cohort a skos:Concept;
  skos:prefLabel "Cohort"@en;
  skos:definition "Group of beneficiaries that enrolled within a specific time period (only defined for Kenyan beneficiaries).";
  skos:inScheme <http://PharmAccess/MomCare/>;
  skos:topConceptOf <http://PharmAccess/MomCare/> .

MomCare:Is_adult a skos:Concept;
  skos:prefLabel "Is_adult"@en;
  skos:definition "Label derived when age of enrolment is 17 years or above.";
  skos:inScheme <http://PharmAccess/MomCare/>;
  skos:topConceptOf <http://PharmAccess/MomCare/> .

MomCare:Age_group a skos:Concept;
  skos:prefLabel "Age_group"@en;
  skos:definition "Categories derived from age at enrolment.";
  skos:inScheme <http://PharmAccess/MomCare/>;
  skos:topConceptOf <http://PharmAccess/MomCare/> .

MomCare:Enrolment_region a skos:Concept;
  skos:prefLabel "Enrolment_region"@en;
  skos:definition "Region of enrolment in MomCare program.";
  skos:inScheme <http://PharmAccess/MomCare/>;
  skos:topConceptOf <http://PharmAccess/MomCare/> .

MomCare:Enrolment_date a skos:Concept;
  skos:prefLabel "Enrolment_date"@en;
  skos:definition "Date of enrolment in MomCare program. This date is sometimes manually adjusted to allow beneficiaries to qualify for enrolment.";
  skos:inScheme <http://PharmAccess/MomCare/>;
  skos:topConceptOf <http://PharmAccess/MomCare/> .

MomCare:program_id a skos:Concept;
  skos:prefLabel "program_id"@en;
  skos:definition "Identifier of time period and specific rules of MomCare program";
  skos:inScheme <http://PharmAccess/MomCare/>;
  skos:topConceptOf <http://PharmAccess/MomCare/> .

MomCare:Enrolment_provider_id a skos:Concept;
  skos:prefLabel "Enrolment_provider_id"@en;
  skos:definition "Identifier of care provider linked to the MomCare program", "Identifier of care provider linked to the MomCare program.";
  skos:inScheme <http://PharmAccess/MomCare/>;
  skos:topConceptOf <http://PharmAccess/MomCare/> .

MomCare:Enrolment_provider_name a skos:Concept;
  skos:prefLabel "Enrolment_provider_name"@en;
  skos:definition "Name of care provider linked to the MomCare program.";
  skos:inScheme <http://PharmAccess/MomCare/>;
  skos:topConceptOf <http://PharmAccess/MomCare/> .

MomCare:Enrolment_week a skos:Concept;
  skos:prefLabel "Enrolment_week"@en;
  skos:definition "Week of enrolment in MomCare program in terms of pregnancy. Calculated by setting estimated delivery date at 40 weeks and taking the difference with the enrolment date in weeks.";
  skos:inScheme <http://PharmAccess/MomCare/>;
  skos:topConceptOf <http://PharmAccess/MomCare/> .

MomCare:Risk_level a skos:Concept;
  skos:prefLabel "Risk_level"@en;
  skos:definition "Label derived from diagnosis or age level risk factors.";
  skos:inScheme <http://PharmAccess/MomCare/>;
  skos:topConceptOf <http://PharmAccess/MomCare/> .

MomCare:Enrolment_trimester a skos:Concept;
  skos:prefLabel "Enrolment_trimester"@en;
  skos:definition "Trimester of enrolment in MomCare program in terms of pregnancy. Calculated by taking the enrolment week.";
  skos:inScheme <http://PharmAccess/MomCare/>;
  skos:topConceptOf <http://PharmAccess/MomCare/> .

MomCare:Week_risk_detection a skos:Concept;
  skos:prefLabel "Week_risk_detection"@en;
  skos:definition "Week that risk label was given. Calculated by setting estimated delivery date at 40 weeks and taking the difference with the risk attribution date in weeks.";
  skos:inScheme <http://PharmAccess/MomCare/>;
  skos:topConceptOf <http://PharmAccess/MomCare/> .

MomCare:Risk_factors a skos:Concept;
  skos:prefLabel "Risk_factors"@en;
  skos:definition "Summary of diagnosis and age categorizations that contribute to risk level.";
  skos:inScheme <http://PharmAccess/MomCare/>;
  skos:topConceptOf <http://PharmAccess/MomCare/> .

MomCare:Current_week a skos:Concept;
  skos:prefLabel "Current_week"@en;
  skos:definition "Current week in MomCare program in terms of pregnancy. Calculated by setting estimated delivery date at 40 weeks and taking the difference with the current date in weeks.";
  skos:inScheme <http://PharmAccess/MomCare/>;
  skos:topConceptOf <http://PharmAccess/MomCare/> .

MomCare:Expected_delivery_date a skos:Concept;
  skos:prefLabel "Expected_delivery_date"@en;
  skos:definition "Expected delivery date of beneficiary identified at enrolment. Estimate usually based on menstruation cycle and estimate by beneficiary about conception timing.";
  skos:inScheme <http://PharmAccess/MomCare/>;
  skos:topConceptOf <http://PharmAccess/MomCare/> .

MomCare:Actual_delivery_date a skos:Concept;
  skos:prefLabel "Actual_delivery_date"@en;
  skos:definition "Actual date of delivery.";
  skos:inScheme <http://PharmAccess/MomCare/>;
  skos:topConceptOf <http://PharmAccess/MomCare/> .

MomCare:Delivery_type a skos:Concept;
  skos:prefLabel "Delivery_type"@en;
  skos:definition "Delivery that can be categorized as c-section or normal (via birth canal).",
    <http://PharmAccess/MomCare/#%20Hongera%20kwa%20kujifungua%20salama.%20Je%20umejifungua%20kwa%20njia%20gani?>,
    "14. How did you deliver?";
  skos:inScheme <http://PharmAccess/MomCare/>;
  skos:topConceptOf <http://PharmAccess/MomCare/> .

MomCare:Date_finished a skos:Concept;
  skos:prefLabel "Date_finished"@en;
  skos:definition "Date of unenrolment from MomCare program. This date is manually set 60 weeks after the enrolment date.";
  skos:inScheme <http://PharmAccess/MomCare/>;
  skos:topConceptOf <http://PharmAccess/MomCare/> .

MomCare:Ancs a skos:Concept;
  skos:prefLabel "Ancs"@en;
  skos:definition "Count of visits categorized as antenatal care visits within enrolment period.";
  skos:inScheme <http://PharmAccess/MomCare/>;
  skos:topConceptOf <http://PharmAccess/MomCare/> .

MomCare:Delivery a skos:Concept;
  skos:prefLabel "Delivery"@en;
  skos:definition "Count of delivery visits within enrolment period.";
  skos:inScheme <http://PharmAccess/MomCare/>;
  skos:topConceptOf <http://PharmAccess/MomCare/> .

MomCare:Pncs a skos:Concept;
  skos:prefLabel "Pncs"@en;
  skos:definition "Count of visits categorized as postnatal care visits within enrolment period.";
  skos:inScheme <http://PharmAccess/MomCare/>;
  skos:topConceptOf <http://PharmAccess/MomCare/> .

MomCare:Imms a skos:Concept;
  skos:prefLabel "Imms"@en;
  skos:definition "Count of visits categorized as immunization visits within enrolment period.";
  skos:inScheme <http://PharmAccess/MomCare/>;
  skos:topConceptOf <http://PharmAccess/MomCare/> .

MomCare:Delivery_out a skos:Concept;
  skos:prefLabel "Delivery_out"@en;
  skos:definition "Label if delivered is registered to have occurred but not with a MomCare registered provider.";
  skos:inScheme <http://PharmAccess/MomCare/>;
  skos:topConceptOf <http://PharmAccess/MomCare/> .

MomCare:Diagnoses a skos:Concept;
  skos:prefLabel "Diagnoses"@en;
  skos:definition "Summary of diagnoses derived from diagnosis files and linked to beneficiary.";
  skos:inScheme <http://PharmAccess/MomCare/>;
  skos:topConceptOf <http://PharmAccess/MomCare/> .

MomCare:Total_costs a skos:Concept;
  skos:prefLabel "Total_costs"@en;
  skos:definition "Sum of costs derived from billing items linked to beneficiary.";
  skos:inScheme <http://PharmAccess/MomCare/>;
  skos:topConceptOf <http://PharmAccess/MomCare/> .

MomCare:Total_costs_eur a skos:Concept;
  skos:prefLabel "Total_costs_eur"@en;
  skos:definition "Sum of costs converted to euros derived from billing items linked to beneficiary.";
  skos:inScheme <http://PharmAccess/MomCare/>;
  skos:topConceptOf <http://PharmAccess/MomCare/> .

MomCare:Journey_score a skos:Concept;
  skos:prefLabel "Journey_score"@en;
  skos:definition "Score of care journey based on calculation specified at https://pharmaccess.atlassian.net/wiki/spaces/MOM/pages/1990852646/Business+rules";
  skos:inScheme <http://PharmAccess/MomCare/>;
  skos:topConceptOf <http://PharmAccess/MomCare/> .

MomCare:Dbt_recency_value a skos:Concept;
  skos:prefLabel "Dbt_recency_value"@en;
  skos:definition "Administrative value.";
  skos:inScheme <http://PharmAccess/MomCare/>;
  skos:topConceptOf <http://PharmAccess/MomCare/> .

MomCare:Dwh_inserttime a skos:Concept;
  skos:prefLabel "Dwh_inserttime"@en;
  skos:definition "Administrative time.";
  skos:inScheme <http://PharmAccess/MomCare/>;
  skos:topConceptOf <http://PharmAccess/MomCare/> .

MomCare:enrolment_survey a skos:Concept;
  skos:prefLabel "enrolment_survey"@en;
  skos:definition "This is a set of controlled terms for the Enrolment Survey.";
  skos:inScheme <http://PharmAccess/MomCare/>;
  skos:topConceptOf <http://PharmAccess/MomCare/> .

MomCare:Pregnancy_age_first_time a skos:Concept;
  skos:prefLabel "Pregnancy_age_first_time"@en;
  skos:definition "At what age did you have your first child?";
  skos:inScheme <http://PharmAccess/MomCare/>;
  skos:topConceptOf <http://PharmAccess/MomCare/> .

MomCare:Ability_read_write a skos:Concept;
  skos:prefLabel "Ability_read_write"@en;
  skos:definition "Can you write and read in any language?";
  skos:inScheme <http://PharmAccess/MomCare/>;
  skos:topConceptOf <http://PharmAccess/MomCare/> .

MomCare:Clinic_visit_current_pregnancy_before a skos:Concept;
  skos:prefLabel "Clinic_visit_current_pregnancy_before"@en;
  skos:definition "Did you already visit another clinic during this pregnancy? / Have you already had any ANC visits during this pregnancy?";
  skos:inScheme <http://PharmAccess/MomCare/>;
  skos:topConceptOf <http://PharmAccess/MomCare/> .

MomCare:Clinic_visit_previous_pregnancy a skos:Concept;
  skos:prefLabel "Clinic_visit_previous_pregnancy"@en;
  skos:definition "Did you attend a clinic during your previous pregnancy for delivery and/or check-ups?(If yes, please select all that apply) / Did you attend a health facility during your previous pregnancy for any of the following services?";
  skos:inScheme <http://PharmAccess/MomCare/>;
  skos:topConceptOf <http://PharmAccess/MomCare/> .

MomCare:Complications_previous_pregnancy a skos:Concept;
  skos:prefLabel "Complications_previous_pregnancy"@en;
  skos:definition "Did you have any of these complications in your previous pregnancies? (If yes, please select all that apply) / (Past medical history)Did you have any of these complications in your previous pregnancies?";
  skos:inScheme <http://PharmAccess/MomCare/>;
  skos:topConceptOf <http://PharmAccess/MomCare/> .

MomCare:Existing_health_conditions a skos:Concept;
  skos:prefLabel "Existing_health_conditions"@en;
  skos:definition "Do you have any of these health conditions? (Please select all that apply) / Do you have, or have you had any of these health conditions?";
  skos:inScheme <http://PharmAccess/MomCare/>;
  skos:topConceptOf <http://PharmAccess/MomCare/> .

MomCare:Household_television a skos:Concept;
  skos:prefLabel "Household_television"@en;
  skos:definition "Does this household have a functional television or Pay TV? / Does your household have a television?";
  skos:inScheme <http://PharmAccess/MomCare/>;
  skos:topConceptOf <http://PharmAccess/MomCare/> .

MomCare:Household_electricity a skos:Concept;
  skos:prefLabel "Household_electricity"@en;
  skos:definition "Does your household have electricity?";
  skos:inScheme <http://PharmAccess/MomCare/>;
  skos:topConceptOf <http://PharmAccess/MomCare/> .

MomCare:Pregnancy_history a skos:Concept;
  skos:prefLabel "Pregnancy_history"@en;
  skos:definition "Have you been pregnant before?";
  skos:inScheme <http://PharmAccess/MomCare/>;
  skos:topConceptOf <http://PharmAccess/MomCare/> .

MomCare:Travel_time a skos:Concept;
  skos:prefLabel "Travel_time"@en;
  skos:definition "How long do you have to travel to reach this clinic (in minutes)? / How long do you have to travel to reach this clinic (in hours)?";
  skos:inScheme <http://PharmAccess/MomCare/>;
  skos:topConceptOf <http://PharmAccess/MomCare/> .

MomCare:Pregnancy_children_birth_number a skos:Concept;
  skos:prefLabel "Pregnancy_children_birth_number"@en;
  skos:definition "How many children have you given birth to before?";
  skos:inScheme <http://PharmAccess/MomCare/>;
  skos:topConceptOf <http://PharmAccess/MomCare/> .

MomCare:Household_persons a skos:Concept;
  skos:prefLabel "Household_persons"@en;
  skos:definition "How many people are in your household?";
  skos:inScheme <http://PharmAccess/MomCare/>;
  skos:topConceptOf <http://PharmAccess/MomCare/> .

MomCare:Social_support_persons a skos:Concept;
  skos:prefLabel "Social_support_persons"@en;
  skos:definition "How many people do you have near you that you can readily count on for help in time of difficulty or when you are sick? / How many people do you have near you that you can readily count for help in time of difficulty or when you are sick?";
  skos:inScheme <http://PharmAccess/MomCare/>;
  skos:topConceptOf <http://PharmAccess/MomCare/> .

MomCare:Household_rooms a skos:Concept;
  skos:prefLabel "Household_rooms"@en;
  skos:definition "How many rooms does this household occupy?(DO NOT COUNT BATHROOMS, TOILETS, STOREROOMS OR GARAGES)";
  skos:inScheme <http://PharmAccess/MomCare/>;
  skos:topConceptOf <http://PharmAccess/MomCare/> .

MomCare:Pregnancy_history_amount_before a skos:Concept;
  skos:prefLabel "Pregnancy_history_amount_before"@en;
  skos:definition "How many times have you been pregnant before?";
  skos:inScheme <http://PharmAccess/MomCare/>;
  skos:topConceptOf <http://PharmAccess/MomCare/> .

MomCare:Pregnancy_history_amount a skos:Concept;
  skos:prefLabel "Pregnancy_history_amount"@en;
  skos:definition "How many times have you been pregnant? / How many times have you been pregnant before?";
  skos:inScheme <http://PharmAccess/MomCare/>;
  skos:topConceptOf <http://PharmAccess/MomCare/> .

MomCare:Household_hunger_pastyear a skos:Concept;
  skos:prefLabel "Household_hunger_pastyear"@en;
  skos:definition "In the last 12 months, were you or any other household member hungry but did not eat because of lack of money or other resources?";
  skos:inScheme <http://PharmAccess/MomCare/>;
  skos:topConceptOf <http://PharmAccess/MomCare/> .

MomCare:Mental_experience_depression a skos:Concept;
  skos:prefLabel "Mental_experience_depression"@en;
  skos:definition "In the last 2 weeks, how often have you been bothered by feeling down, depressed or hopeless?",
    <http://PharmAccess/MomCare/#%20Over%20the%20last%202%20weeks>, "how often have you been bothered by feeling down",
    "depressed", "or hopeless? / MomCare: Kwa wiki mbili zilizopita", "umekua ukipata msongo wa mawazo au kusononeka?";
  skos:inScheme <http://PharmAccess/MomCare/>;
  skos:topConceptOf <http://PharmAccess/MomCare/> .

MomCare:Mental_experience_interest a skos:Concept;
  skos:prefLabel "Mental_experience_interest"@en;
  skos:definition "In the last 2 weeks, how often have you been bothered by little interest or pleasure in doing things?",
    <http://PharmAccess/MomCare/#%20Over%20the%20last%202%20weeks>, "how often have you been bothered by little interest or pleasure in doing things? / MomCare: Kwa wiki mbili zilizopita umepoteza furaha katika kufanya jambo lolote?";
  skos:inScheme <http://PharmAccess/MomCare/>;
  skos:topConceptOf <http://PharmAccess/MomCare/> .

MomCare:Survey_language_choice a skos:Concept;
  skos:prefLabel "Survey_language_choice"@en;
  skos:definition "MomCare will send you SMS survey, responding is free of charge. Do you prefer to receive those in English or Swahili?";
  skos:inScheme <http://PharmAccess/MomCare/>;
  skos:topConceptOf <http://PharmAccess/MomCare/> .

MomCare:Household_airtime_spendperweek a skos:Concept;
  skos:prefLabel "Household_airtime_spendperweek"@en;
  skos:definition "On average, how much does the head of the household spend on airtime in a week?";
  skos:inScheme <http://PharmAccess/MomCare/>;
  skos:topConceptOf <http://PharmAccess/MomCare/> .

MomCare:Existing_health_conditions_other a skos:Concept;
  skos:prefLabel "Existing_health_conditions_other"@en;
  skos:definition "Please describe the OTHER health conditions";
  skos:inScheme <http://PharmAccess/MomCare/>;
  skos:topConceptOf <http://PharmAccess/MomCare/> .

MomCare:Pregnancy_EDD a skos:Concept;
  skos:prefLabel "Pregnancy_EDD"@en;
  skos:definition "What is the estimated date of delivery (EDD)?";
  skos:inScheme <http://PharmAccess/MomCare/>;
  skos:topConceptOf <http://PharmAccess/MomCare/> .

MomCare:Household_educationlevel_head a skos:Concept;
  skos:prefLabel "Household_educationlevel_head"@en;
  skos:definition "What is the highest educational level the household head HAS completed?";
  skos:inScheme <http://PharmAccess/MomCare/>;
  skos:topConceptOf <http://PharmAccess/MomCare/> .

MomCare:Household_material_walls a skos:Concept;
  skos:prefLabel "Household_material_walls"@en;
  skos:definition "What is the main material of the external walls of your dwelling? / What is the main material of the exterior walls of your dwelling?";
  skos:inScheme <http://PharmAccess/MomCare/>;
  skos:topConceptOf <http://PharmAccess/MomCare/> .

MomCare:Household_material_floor a skos:Concept;
  skos:prefLabel "Household_material_floor"@en;
  skos:definition "What is the main material of the floor of your dwelling?";
  skos:inScheme <http://PharmAccess/MomCare/>;
  skos:topConceptOf <http://PharmAccess/MomCare/> .

MomCare:Household_material_roof a skos:Concept;
  skos:prefLabel "Household_material_roof"@en;
  skos:definition "What is the main material of the roof of your dwelling?";
  skos:inScheme <http://PharmAccess/MomCare/>;
  skos:topConceptOf <http://PharmAccess/MomCare/> .

MomCare:Household_fuel_cooking a skos:Concept;
  skos:prefLabel "Household_fuel_cooking"@en;
  skos:definition "What type of fuel does your household mainly use for cooking?";
  skos:inScheme <http://PharmAccess/MomCare/>;
  skos:topConceptOf <http://PharmAccess/MomCare/> .

MomCare:Household_toilet_type a skos:Concept;
  skos:prefLabel "Household_toilet_type"@en;
  skos:definition "What type of toilet facility do members of your household usually use?";
  skos:inScheme <http://PharmAccess/MomCare/>;
  skos:topConceptOf <http://PharmAccess/MomCare/> .

MomCare:Travel_means a skos:Concept;
  skos:prefLabel "Travel_means"@en;
  skos:definition "Which means of transport do you use?";
  skos:inScheme <http://PharmAccess/MomCare/>;
  skos:topConceptOf <http://PharmAccess/MomCare/> .

MomCare:Clinic_referral_source a skos:Concept;
  skos:prefLabel "Clinic_referral_source"@en;
  skos:definition "Who referred you to this clinic?";
  skos:inScheme <http://PharmAccess/MomCare/>;
  skos:topConceptOf <http://PharmAccess/MomCare/> .

MomCare:Household_radio a skos:Concept;
  skos:prefLabel "Household_radio"@en;
  skos:definition "Does your household have a radio?";
  skos:inScheme <http://PharmAccess/MomCare/>;
  skos:topConceptOf <http://PharmAccess/MomCare/> .

MomCare:Household_iron a skos:Concept;
  skos:prefLabel "Household_iron"@en;
  skos:definition "Does your household have an iron?";
  skos:inScheme <http://PharmAccess/MomCare/>;
  skos:topConceptOf <http://PharmAccess/MomCare/> .

MomCare:Household_bankaccount a skos:Concept;
  skos:prefLabel "Household_bankaccount"@en;
  skos:definition "Does any member of this household have a bank account?";
  skos:inScheme <http://PharmAccess/MomCare/>;
  skos:topConceptOf <http://PharmAccess/MomCare/> .

MomCare:Household_source_energy a skos:Concept;
  skos:prefLabel "Household_source_energy"@en;
  skos:definition "What is the main source of energy for lighting in the household?";
  skos:inScheme <http://PharmAccess/MomCare/>;
  skos:topConceptOf <http://PharmAccess/MomCare/> .

MomCare:Height a skos:Concept;
  skos:prefLabel "Height"@en;
  skos:definition "Height:";
  skos:inScheme <http://PharmAccess/MomCare/>;
  skos:topConceptOf <http://PharmAccess/MomCare/> .

MomCare:Obstetric_history a skos:Concept;
  skos:prefLabel "Obstetric_history"@en;
  skos:definition "Obstetric History:";
  skos:inScheme <http://PharmAccess/MomCare/>;
  skos:topConceptOf <http://PharmAccess/MomCare/> .

MomCare:Lifestyle_smokedrinkdrugs a skos:Concept;
  skos:prefLabel "Lifestyle_smokedrinkdrugs"@en;
  skos:definition "Do you smoke, drink alcohol or use drugs?";
  skos:inScheme <http://PharmAccess/MomCare/>;
  skos:topConceptOf <http://PharmAccess/MomCare/> .

MomCare:sms_survey a skos:Concept;
  skos:prefLabel "sms_survey"@en;
  skos:inScheme <http://PharmAccess/MomCare/>;
  skos:topConceptOf <http://PharmAccess/MomCare/> .

MomCare:Household_chronic_condition a skos:Concept;
  skos:prefLabel "Household_chronic_condition"@en;
  skos:definition "Do you or any household member have a chronic medical condition?";
  skos:inScheme <http://PharmAccess/MomCare/>;
  skos:topConceptOf <http://PharmAccess/MomCare/> .

MomCare:Breastfeeding_yesno a skos:Concept;
  skos:prefLabel "Breastfeeding_yesno"@en;
  skos:definition "Do you plan to breastfeed your baby when he or she is born? 1= No 2= Yes";
  skos:inScheme <http://PharmAccess/MomCare/>;
  skos:topConceptOf <http://PharmAccess/MomCare/> .

MomCare:Improve_services a skos:Concept;
  skos:prefLabel "Improve_services"@en;
  skos:definition "How can we improve the services you received?";
  skos:inScheme <http://PharmAccess/MomCare/>;
  skos:topConceptOf <http://PharmAccess/MomCare/> .

MomCare:Improve_comfort a skos:Concept;
  skos:prefLabel "Improve_comfort"@en;
  skos:definition "How can we improve to make you more comfortable with the care you receive?";
  skos:inScheme <http://PharmAccess/MomCare/>;
  skos:topConceptOf <http://PharmAccess/MomCare/> .

MomCare:Breastfeeding_confidence a skos:Concept;
  skos:prefLabel "Breastfeeding_confidence"@en;
  skos:definition "How confident do you feel about breast feeding? 1 = Not at all confident 2 = Not very confident 3 = Somewhat confident 4 = Confident 5 = Very confident",
    "29. How confident are you with breastfeeding?";
  skos:inScheme <http://PharmAccess/MomCare/>;
  skos:topConceptOf <http://PharmAccess/MomCare/> .

MomCare:Breastfeeding_confidence_spaces a skos:Concept;
  skos:prefLabel "Breastfeeding_confidence_spaces"@en;
  skos:definition "How confident do you feel about breast feeding?n1 = Not at all confidentn2 = Not very confidentn3 = Somewhat confidentn4 = Confidentn5 = Very confident";
  skos:inScheme <http://PharmAccess/MomCare/>;
  skos:topConceptOf <http://PharmAccess/MomCare/> .

MomCare:Household_adults a skos:Concept;
  skos:prefLabel "Household_adults"@en;
  skos:definition "How many adults live in your household?";
  skos:inScheme <http://PharmAccess/MomCare/>;
  skos:topConceptOf <http://PharmAccess/MomCare/> .

MomCare:Household_children a skos:Concept;
  skos:prefLabel "Household_children"@en;
  skos:definition "How many children live in your household? (FOR NONE PUT 0)";
  skos:inScheme <http://PharmAccess/MomCare/>;
  skos:topConceptOf <http://PharmAccess/MomCare/> .

MomCare:Role_preparation a skos:Concept;
  skos:prefLabel "Role_preparation"@en;
  skos:definition "How prepared do you feel about looking after your baby? 0 = Very much 1 = A lot 2 = A little 3 = Not at all";
  skos:inScheme <http://PharmAccess/MomCare/>;
  skos:topConceptOf <http://PharmAccess/MomCare/> .

MomCare:Role_preparation_spaces a skos:Concept;
  skos:prefLabel "Role_preparation_spaces"@en;
  skos:definition "How prepared do you feel about looking after your baby?n0 = Very muchn1 = A lotn2 = A littlen3 = Not at all";
  skos:inScheme <http://PharmAccess/MomCare/>;
  skos:topConceptOf <http://PharmAccess/MomCare/> .

MomCare:Experience_lamazeclass a skos:Concept;
  skos:prefLabel "Experience_lamazeclass"@en;
  skos:definition "How satisfied were you with the Lamaze class? 0 = Very unsatisfied 1 = Unsatisfied 2 = Neither satisfied nor dissatisfied 3 = Satisfied 4 = Very satisfied";
  skos:inScheme <http://PharmAccess/MomCare/>;
  skos:topConceptOf <http://PharmAccess/MomCare/> .

MomCare:Social_satisfaction a skos:Concept;
  skos:prefLabel "Social_satisfaction"@en;
  skos:definition "In general, how would you rate your satisfaction with your social activities and relationships? 5 = Excellent 4 = Very good 3 = Good 2 = Fair 1 = Poor";
  skos:inScheme <http://PharmAccess/MomCare/>;
  skos:topConceptOf <http://PharmAccess/MomCare/> .

MomCare:Quality_of_life a skos:Concept;
  skos:prefLabel "Quality_of_life"@en;
  skos:definition "In general, would you say your quality of life is: 5 = Excellent 4 = Very good 3 = Good 2 = Fair 1 = Poor";
  skos:inScheme <http://PharmAccess/MomCare/>;
  skos:topConceptOf <http://PharmAccess/MomCare/> .

MomCare:Quality_of_life_spaces a skos:Concept;
  skos:prefLabel "Quality_of_life_spaces"@en;
  skos:definition "In general, would you say your quality of life is:n5 = Excellentn4 = Very goodn3 = Goodn2 = Fairn1 = Poor";
  skos:inScheme <http://PharmAccess/MomCare/>;
  skos:topConceptOf <http://PharmAccess/MomCare/> .

MomCare:Residence_county a skos:Concept;
  skos:prefLabel "Residence_county"@en;
  skos:definition "In which County do you live?";
  skos:inScheme <http://PharmAccess/MomCare/>;
  skos:topConceptOf <http://PharmAccess/MomCare/> .

MomCare:Improve_experience_like_dislike_postnatal a skos:Concept;
  skos:prefLabel "Improve_experience_like_dislike_postnatal"@en;
  skos:definition <http://PharmAccess/MomCare/#%20Congratulations%20on%20your%20baby!%20Please%20tell%20us%20one%20thing%20you%20liked%20and%20one%20thing%20you%20did%20not%20like%20about%20the%20care%20received?>;
  skos:inScheme <http://PharmAccess/MomCare/>;
  skos:topConceptOf <http://PharmAccess/MomCare/> .

MomCare:Information_next_visit a skos:Concept;
  skos:prefLabel "Information_next_visit"@en;
  skos:definition <http://PharmAccess/MomCare/#%20Did%20the%20clinic%20tell%20you%20when%20to%20visit%20next%20time?>;
  skos:inScheme <http://PharmAccess/MomCare/>;
  skos:topConceptOf <http://PharmAccess/MomCare/> .

MomCare:Breastfeeding_support_received a skos:Concept;
  skos:prefLabel "Breastfeeding_support_received"@en;
  skos:definition <http://PharmAccess/MomCare/#%20Did%20you%20receive%20support%20for%20breastfeeding%20from%20the%20clinic?>;
  skos:inScheme <http://PharmAccess/MomCare/>;
  skos:topConceptOf <http://PharmAccess/MomCare/> .

MomCare:Improve_service_clinic a skos:Concept;
  skos:prefLabel "Improve_service_clinic"@en;
  skos:definition <http://PharmAccess/MomCare/#%20How%20can%20the%20clinic%20improve%20their%20service?%20Your%20feedback%20will%20be%20handled%20anonymously.>;
  skos:inScheme <http://PharmAccess/MomCare/>;
  skos:topConceptOf <http://PharmAccess/MomCare/> .

MomCare:Improve_service_clinic_2 a skos:Concept;
  skos:prefLabel "Improve_service_clinic_2"@en;
  skos:definition <http://PharmAccess/MomCare/#%20How%20can%20we%20improve%20the%20services%20you%20received?>;
  skos:inScheme <http://PharmAccess/MomCare/>;
  skos:topConceptOf <http://PharmAccess/MomCare/> .

MomCare:Improve_experience_like_dislike a skos:Concept;
  skos:prefLabel "Improve_experience_like_dislike"@en;
  skos:definition <http://PharmAccess/MomCare/#%20Please%20tell%20us%20one%20thing%20you%20liked%20and%20one%20thing%20you%20did%20not%20like%20about%20the%20care%20received%20during%20delivery?>;
  skos:inScheme <http://PharmAccess/MomCare/>;
  skos:topConceptOf <http://PharmAccess/MomCare/> .

MomCare:Improve_experience_like_dislike_2 a skos:Concept;
  skos:prefLabel "Improve_experience_like_dislike_2"@en;
  skos:definition <http://PharmAccess/MomCare/#%20Thank%20you%20#name#%20for%20being%20part%20of%20MomCare%20so%20far!%20Please%20tell%20us%20one%20thing%20you%20liked%20and%20one%20thing%20you%20didn%20t%20like?>;
  skos:inScheme <http://PharmAccess/MomCare/>;
  skos:topConceptOf <http://PharmAccess/MomCare/> .

MomCare:Improve_experience_like_dislike_registration a skos:Concept;
  skos:prefLabel "Improve_experience_like_dislike_registration"@en;
  skos:definition <http://PharmAccess/MomCare/#%20Thank%20you%20#name#%20for%20joining%20MomCare.%20Please%20write%20one%20thing%20you%20liked%20and%20one%20thing%20you%20didn%20t%20like%20about%20the%20registration%20process?>;
  skos:inScheme <http://PharmAccess/MomCare/>;
  skos:topConceptOf <http://PharmAccess/MomCare/> .

MomCare:Service_satisfaction a skos:Concept;
  skos:prefLabel "Service_satisfaction"@en;
  skos:definition <http://PharmAccess/MomCare/#%20Thank%20you%20#name#%20for%20visiting%20the%20clinic.%20Were%20you%20satisfied%20with%20the%20service?>;
  skos:inScheme <http://PharmAccess/MomCare/>;
  skos:topConceptOf <http://PharmAccess/MomCare/> .

MomCare:Service_comfort a skos:Concept;
  skos:prefLabel "Service_comfort"@en;
  skos:definition <http://PharmAccess/MomCare/#%20Thank%20you%20for%20being%20part%20of%20MomCare%20so%20far!%20Did%20you%20feel%20comfortable%20with%20the%20care%20you%20received%20so%20far?>;
  skos:inScheme <http://PharmAccess/MomCare/>;
  skos:topConceptOf <http://PharmAccess/MomCare/> .

MomCare:Improve_experience_like_dislike_delivery a skos:Concept;
  skos:prefLabel "Improve_experience_like_dislike_delivery"@en;
  skos:definition <http://PharmAccess/MomCare/#%20Well%20done%20#name#%20for%20delivering%20at%20the%20clinic!%20Please%20tell%20us%20one%20thing%20you%20liked%20and%20one%20thing%20you%20did%20not%20like%20about%20the%20care%20received?>;
  skos:inScheme <http://PharmAccess/MomCare/>;
  skos:topConceptOf <http://PharmAccess/MomCare/> .

MomCare:Delivery_respect a skos:Concept;
  skos:prefLabel "Delivery_respect"@en;
  skos:definition <http://PharmAccess/MomCare/#%20Were%20you%20treated%20with%20respect%20during%20delivery?>;
  skos:inScheme <http://PharmAccess/MomCare/>;
  skos:topConceptOf <http://PharmAccess/MomCare/> .

MomCare:Delivery_wellhandled a skos:Concept;
  skos:prefLabel "Delivery_wellhandled"@en;
  skos:definition <http://PharmAccess/MomCare/#%20Were%20you%20well-handled%20during%20your%20time%20of%20delivery?>;
  skos:inScheme <http://PharmAccess/MomCare/>;
  skos:topConceptOf <http://PharmAccess/MomCare/> .

MomCare:Breastfeeding_currentmode a skos:Concept;
  skos:prefLabel "Breastfeeding_currentmode"@en;
  skos:definition "Momcare: Which breastfeeding mode are you currently in?";
  skos:inScheme <http://PharmAccess/MomCare/>;
  skos:topConceptOf <http://PharmAccess/MomCare/> .

MomCare:Breastfeeding_preference a skos:Concept;
  skos:prefLabel "Breastfeeding_preference"@en;
  skos:definition <http://PharmAccess/MomCare/#%20Which%20breastfeeding%20mode%20will%20you%20prefer?>;
  skos:inScheme <http://PharmAccess/MomCare/>;
  skos:topConceptOf <http://PharmAccess/MomCare/> .

MomCare:Delivery_out_where a skos:Concept;
  skos:prefLabel "Delivery_out_where"@en;
  skos:definition <http://PharmAccess/MomCare/#%20Your%20due%20date%20has%20passed>,
    "and your health facility did not see you for your delivery. Kindly answer: Where did you deliver?";
  skos:inScheme <http://PharmAccess/MomCare/>;
  skos:topConceptOf <http://PharmAccess/MomCare/> .

MomCare:Service_satisfaction_secondclinic a skos:Concept;
  skos:prefLabel "Service_satisfaction_secondclinic"@en;
  skos:definition "Well done for going for your second clinic. Were you satisfied with the service?";
  skos:inScheme <http://PharmAccess/MomCare/>;
  skos:topConceptOf <http://PharmAccess/MomCare/> .

MomCare:Improve_experience_how a skos:Concept;
  skos:prefLabel "Improve_experience_how"@en;
  skos:definition "What can we do to improve it?";
  skos:inScheme <http://PharmAccess/MomCare/>;
  skos:topConceptOf <http://PharmAccess/MomCare/> .

MomCare:Role_feelings a skos:Concept;
  skos:prefLabel "Role_feelings"@en;
  skos:definition "What feelings do you have towards your child? 1. Resentful 2. Dislike 3. Neutral or nothing 4. Joyful 5. Disappointed 6. Aggressive";
  skos:inScheme <http://PharmAccess/MomCare/>;
  skos:topConceptOf <http://PharmAccess/MomCare/> .

MomCare:Service_like_1 a skos:Concept;
  skos:prefLabel "Service_like_1"@en;
  skos:definition <http://PharmAccess/MomCare/#%20Tafadhali%20andika%20kitu%20kilichokufurahisha?>;
  skos:inScheme <http://PharmAccess/MomCare/>;
  skos:topConceptOf <http://PharmAccess/MomCare/> .

MomCare:Recommend_to_others a skos:Concept;
  skos:prefLabel "Recommend_to_others"@en;
  skos:definition <http://PharmAccess/MomCare/#%20Kulinganisha%20huduma%20umekuwa%20ukipewa>,
    "je unaweza kumshauri mtu mwingine kuja kituo hiki?";
  skos:inScheme <http://PharmAccess/MomCare/>;
  skos:topConceptOf <http://PharmAccess/MomCare/> .

MomCare:Service_payment a skos:Concept;
  skos:prefLabel "Service_payment"@en;
  skos:definition <http://PharmAccess/MomCare/#%20Je>, "uliambiwa kulipia huduma yeyote kipindi cha kujifungua?";
  skos:inScheme <http://PharmAccess/MomCare/>;
  skos:topConceptOf <http://PharmAccess/MomCare/> .

MomCare:Service_satisfaction_1 a skos:Concept;
  skos:prefLabel "Service_satisfaction_1"@en;
  skos:definition <http://PharmAccess/MomCare/#%20Je%20ulifurahishwa%20na%20huduma%20ulizopewa?>;
  skos:inScheme <http://PharmAccess/MomCare/>;
  skos:topConceptOf <http://PharmAccess/MomCare/> .

MomCare:Breastfeeding_mode a skos:Concept;
  skos:prefLabel "Breastfeeding_mode"@en;
  skos:definition <http://PharmAccess/MomCare/#%20Je%20ulifanikiwa%20kumnyonyesha%20mtoto%20kwa:>,
    "28. How did you feed your child in the first 6 months?";
  skos:inScheme <http://PharmAccess/MomCare/>;
  skos:topConceptOf <http://PharmAccess/MomCare/> .

MomCare:Service_payment_what a skos:Concept;
  skos:prefLabel "Service_payment_what"@en;
  skos:definition <http://PharmAccess/MomCare/#%20Je>, "ulilipa shilingi ngapi? Na ni kwa ajili ya nini?";
  skos:inScheme <http://PharmAccess/MomCare/>;
  skos:topConceptOf <http://PharmAccess/MomCare/> .

MomCare:Feedback_consent_1 a skos:Concept;
  skos:prefLabel "Feedback_consent_1"@en;
  skos:definition "Tungependa kukuuliza maswali kadhaa juu ya ubora wa huduma ulizopokea kituoni. Kujibu maswali ni bure. Tunaweza kuendelea?";
  skos:inScheme <http://PharmAccess/MomCare/>;
  skos:topConceptOf <http://PharmAccess/MomCare/> .

MomCare:Breastfeeding_time a skos:Concept;
  skos:prefLabel "Breastfeeding_time"@en;
  skos:definition <http://PharmAccess/MomCare/#%20Je%20una%20mpango%20wa%20kunyonyesha%20mtoto%20kwa:>;
  skos:inScheme <http://PharmAccess/MomCare/>;
  skos:topConceptOf <http://PharmAccess/MomCare/> .

MomCare:Feedback_consent a skos:Concept;
  skos:prefLabel "Feedback_consent"@en;
  skos:definition <http://PharmAccess/MomCare/#%20Hongera%20kwa%20kuhudhuria%20cliniki.%20Tunaomba%20kukuuliza%20maswali%20juu%20ya%20ubora%20wa%20huduma%20ulizopata%20kituoni.%20Kujibu%20maswali%20ni%20bure.%20Tunaweza%20kuendelea?>;
  skos:inScheme <http://PharmAccess/MomCare/>;
  skos:topConceptOf <http://PharmAccess/MomCare/> .

MomCare:Service_satisfaction_2 a skos:Concept;
  skos:prefLabel "Service_satisfaction_2"@en;
  skos:definition <http://PharmAccess/MomCare/#%20Je%20ulifurahishwa%20na%20huduma%20ulizokuwa%20unapewa%20kipindi%20cha%20ujazito%20wako?>;
  skos:inScheme <http://PharmAccess/MomCare/>;
  skos:topConceptOf <http://PharmAccess/MomCare/> .

MomCare:Care_usage_tests a skos:Concept;
  skos:prefLabel "Care_usage_tests"@en;
  skos:definition "Momcare: Je Umepimwa vipimo vifuatavyo leo ulipoenda kliniki?";
  skos:inScheme <http://PharmAccess/MomCare/>;
  skos:topConceptOf <http://PharmAccess/MomCare/> .

MomCare:Service_like_2 a skos:Concept;
  skos:prefLabel "Service_like_2"@en;
  skos:definition <http://PharmAccess/MomCare/#%20Tafadhali%20andika%20kitu%20ambacho%20ulikipenda%20ulipohudhuria%20kliniki?>;
  skos:inScheme <http://PharmAccess/MomCare/>;
  skos:topConceptOf <http://PharmAccess/MomCare/> .

MomCare:Service_dislike a skos:Concept;
  skos:prefLabel "Service_dislike"@en;
  skos:definition <http://PharmAccess/MomCare/#%20Tafadhali%20andika%20kitu%20ambacho%20haukukipenda%20ulipohudhuria%20kliniki?>;
  skos:inScheme <http://PharmAccess/MomCare/>;
  skos:topConceptOf <http://PharmAccess/MomCare/> .

MomCare:Care_usage_tests_other a skos:Concept;
  skos:prefLabel "Care_usage_tests_other"@en;
  skos:definition "Tafadhali andika vipimo ambavyo hukupata";
  skos:inScheme <http://PharmAccess/MomCare/>;
  skos:topConceptOf <http://PharmAccess/MomCare/> .

MomCare:Care_usage_services a skos:Concept;
  skos:prefLabel "Care_usage_services"@en;
  skos:definition <http://PharmAccess/MomCare/#%20Chagua%20huduma%20ulizopata%20ulipoenda%20kituo%20cha%20afya>;
  skos:inScheme <http://PharmAccess/MomCare/>;
  skos:topConceptOf <http://PharmAccess/MomCare/> .

MomCare:Service_satisfaction_3 a skos:Concept;
  skos:prefLabel "Service_satisfaction_3"@en;
  skos:definition <http://PharmAccess/MomCare/#%20Asante%20kwa%20kuhudhuria%20kiliniki%20katika%20kituo%20cha%20afya.%20Je>,
    "uliridhika na ubora wa huduma?";
  skos:inScheme <http://PharmAccess/MomCare/>;
  skos:topConceptOf <http://PharmAccess/MomCare/> .

MomCare:Improve_how a skos:Concept;
  skos:prefLabel "Improve_how"@en;
  skos:definition <http://PharmAccess/MomCare/#%20Ni%20jinsi%20gani%20tunaweza%20kuendelea%20kuboresha%20huduma%20za%20afya%20ulizozipata?>;
  skos:inScheme <http://PharmAccess/MomCare/>;
  skos:topConceptOf <http://PharmAccess/MomCare/> .

MomCare:Improve_why a skos:Concept;
  skos:prefLabel "Improve_why"@en;
  skos:definition <http://PharmAccess/MomCare/#%20Tafadhali%20andika%20ni%20kwa%20nini>;
  skos:inScheme <http://PharmAccess/MomCare/>;
  skos:topConceptOf <http://PharmAccess/MomCare/> .

MomCare:Satisfaction_why_not a skos:Concept;
  skos:prefLabel "Satisfaction_why_not"@en;
  skos:definition <http://PharmAccess/MomCare/#%20Kwa%20nini%20hukuridhika%20na%20huduma%20ulizopewa%20kituoni?>;
  skos:inScheme <http://PharmAccess/MomCare/>;
  skos:topConceptOf <http://PharmAccess/MomCare/> .

MomCare:eoj_call a skos:Concept;
  skos:prefLabel "eoj_call"@en;
  skos:inScheme <http://PharmAccess/MomCare/>;
  skos:topConceptOf <http://PharmAccess/MomCare/> .

MomCare:StartingDate a skos:Concept;
  skos:prefLabel "StartingDate"@en;
  skos:definition "Date of interview.";
  skos:inScheme <http://PharmAccess/MomCare/>;
  skos:topConceptOf <http://PharmAccess/MomCare/> .

MomCare:EndingDate a skos:Concept;
  skos:prefLabel "EndingDate"@en;
  skos:definition "End date of interview";
  skos:inScheme <http://PharmAccess/MomCare/>;
  skos:topConceptOf <http://PharmAccess/MomCare/> .

MomCare:InterviewerID a skos:Concept;
  skos:prefLabel "InterviewerID"@en;
  skos:definition "Identifier of interviewer undertaking the end of journey call.";
  skos:inScheme <http://PharmAccess/MomCare/>;
  skos:topConceptOf <http://PharmAccess/MomCare/> .

MomCare:contactid a skos:Concept;
  skos:prefLabel "contactid"@en;
  skos:definition "Identifier of beneficiary enrolled in MomCare program for interview purposes.";
  skos:inScheme <http://PharmAccess/MomCare/>;
  skos:topConceptOf <http://PharmAccess/MomCare/> .

MomCare:Consent_participation a skos:Concept;
  skos:prefLabel "Consent_participation"@en;
  skos:definition "Do you agree to participate in this interview?";
  skos:inScheme <http://PharmAccess/MomCare/>;
  skos:topConceptOf <http://PharmAccess/MomCare/> .

MomCare:Education_level a skos:Concept;
  skos:prefLabel "Education_level"@en;
  skos:definition "1. Which is the highest education level you attained?";
  skos:inScheme <http://PharmAccess/MomCare/>;
  skos:topConceptOf <http://PharmAccess/MomCare/> .

MomCare:Child_alive a skos:Concept;
  skos:prefLabel "Child_alive"@en;
  skos:definition "2. Before we continue further, we would like to know the status of your child. Is your child alive?";
  skos:inScheme <http://PharmAccess/MomCare/>;
  skos:topConceptOf <http://PharmAccess/MomCare/> .

MomCare:Child_age a skos:Concept;
  skos:prefLabel "Child_age"@en;
  skos:definition "3. How old is your child?";
  skos:inScheme <http://PharmAccess/MomCare/>;
  skos:topConceptOf <http://PharmAccess/MomCare/> .

MomCare:Child_age_text a skos:Concept;
  skos:prefLabel "Child_age_text"@en;
  skos:definition "Text 3. How old is your child?";
  skos:inScheme <http://PharmAccess/MomCare/>;
  skos:topConceptOf <http://PharmAccess/MomCare/> .

MomCare:Interview_continue a skos:Concept;
  skos:prefLabel "Interview_continue"@en;
  skos:definition "4. Are you comfortable continuing with the interview?";
  skos:inScheme <http://PharmAccess/MomCare/>;
  skos:topConceptOf <http://PharmAccess/MomCare/> .

MomCare:Child_age_of_death a skos:Concept;
  skos:prefLabel "Child_age_of_death"@en;
  skos:definition "5. At what age did your child pass away? [4 weeks =1month. For a child that passed away at age is less than or equal to 2 weeks then indicate as 0, over 2 weeks round up to 1 month.]";
  skos:inScheme <http://PharmAccess/MomCare/>;
  skos:topConceptOf <http://PharmAccess/MomCare/> .

MomCare:Child_age_of_death_text a skos:Concept;
  skos:prefLabel "Child_age_of_death_text"@en;
  skos:definition "Text 5. At what age did your child pass away? [4 weeks =1month. For a child that passed away at age is less than or equal to 2 weeks then indicate as 0, over 2 weeks round up to 1 month.]";
  skos:inScheme <http://PharmAccess/MomCare/>;
  skos:topConceptOf <http://PharmAccess/MomCare/> .

MomCare:Child_cause_of_death a skos:Concept;
  skos:prefLabel "Child_cause_of_death"@en;
  skos:definition "5a. Are you willing to let us know what caused the death of your baby?";
  skos:inScheme <http://PharmAccess/MomCare/>;
  skos:topConceptOf <http://PharmAccess/MomCare/> .

MomCare:Child_cause_of_death_text a skos:Concept;
  skos:prefLabel "Child_cause_of_death_text"@en;
  skos:definition "Text 5b. Please tell us what was the reason your baby passed away?";
  skos:inScheme <http://PharmAccess/MomCare/>;
  skos:topConceptOf <http://PharmAccess/MomCare/> .

MomCare:Clinic_visit_outside_1 a skos:Concept;
  skos:prefLabel "Clinic_visit_outside_1"@en;
  skos:definition "6. Apart from {facility}, did you go to any other facility for either Antenatal Clinic, Delivery or Postnatal Clinic during your pregnancy with MomCare? : 1";
  skos:inScheme <http://PharmAccess/MomCare/>;
  skos:topConceptOf <http://PharmAccess/MomCare/> .

MomCare:Clinic_visit_outside_n a skos:Concept;
  skos:prefLabel "Clinic_visit_outside_n"@en;
  skos:definition "6n. Apart from {facility} , did you go to any other facility for either Antenatal Clinic, Delivery or Postnatal Clinic during your pregnancy with MomCare? : 1";
  skos:inScheme <http://PharmAccess/MomCare/>;
  skos:topConceptOf <http://PharmAccess/MomCare/> .

MomCare:Clinic_visit_outside_reason a skos:Concept;
  skos:prefLabel "Clinic_visit_outside_reason"@en;
  skos:definition "7. Why did you visit another facility?";
  skos:inScheme <http://PharmAccess/MomCare/>;
  skos:topConceptOf <http://PharmAccess/MomCare/> .

MomCare:Clinic_visit_outside_reason_text a skos:Concept;
  skos:prefLabel "Clinic_visit_outside_reason_text"@en;
  skos:definition "Text 7. Why did you visit another facility?";
  skos:inScheme <http://PharmAccess/MomCare/>;
  skos:topConceptOf <http://PharmAccess/MomCare/> .

MomCare:Hospital_name a skos:Concept;
  skos:prefLabel "Hospital_name"@en;
  skos:definition "Text 8. What was the name of the hospital you attended?";
  skos:inScheme <http://PharmAccess/MomCare/>;
  skos:topConceptOf <http://PharmAccess/MomCare/> .

MomCare:Facility_type_hospital a skos:Concept;
  skos:prefLabel "Facility_type_hospital"@en;
  skos:definition "9. What type of facility was it?";
  skos:inScheme <http://PharmAccess/MomCare/>;
  skos:topConceptOf <http://PharmAccess/MomCare/> .

MomCare:Transport_mode_facility a skos:Concept;
  skos:prefLabel "Transport_mode_facility"@en;
  skos:definition "10. What mode of transport did you use to access the facility?";
  skos:inScheme <http://PharmAccess/MomCare/>;
  skos:topConceptOf <http://PharmAccess/MomCare/> .

MomCare:Facility_type_delivery a skos:Concept;
  skos:prefLabel "Facility_type_delivery"@en;
  skos:definition "11. What type of facility did you deliver in?";
  skos:inScheme <http://PharmAccess/MomCare/>;
  skos:topConceptOf <http://PharmAccess/MomCare/> .

MomCare:Facility_name_delivery a skos:Concept;
  skos:prefLabel "Facility_name_delivery"@en;
  skos:definition "Text 12. What is the name of the facility you delivered in?";
  skos:inScheme <http://PharmAccess/MomCare/>;
  skos:topConceptOf <http://PharmAccess/MomCare/> .

MomCare:Delivery_weeks_along a skos:Concept;
  skos:prefLabel "Delivery_weeks_along"@en;
  skos:definition "Text 13. How far along were you when you delivered? [ If mother doesn't know, ask in relation to due date i.e how many weeks before or after your due date did you deliver, due date is 40 weeks gestation]";
  skos:inScheme <http://PharmAccess/MomCare/>;
  skos:topConceptOf <http://PharmAccess/MomCare/> .

MomCare:Delivery_complications_1 a skos:Concept;
  skos:prefLabel "Delivery_complications_1"@en;
  skos:definition "15. We would like more information about your delivery. Please let us know which of the following statements apply to you : 1";
  skos:inScheme <http://PharmAccess/MomCare/>;
  skos:topConceptOf <http://PharmAccess/MomCare/> .

MomCare:Information_pregnancy a skos:Concept;
  skos:prefLabel "Information_pregnancy"@en;
  skos:definition "16. Were you given any information about pregnancy danger signs from a doctor or nurse? You can give examples like: less movements of the baby, headache, swollen lower limbs, blood loss";
  skos:inScheme <http://PharmAccess/MomCare/>;
  skos:topConceptOf <http://PharmAccess/MomCare/> .

MomCare:ANC_booklet a skos:Concept;
  skos:prefLabel "ANC_booklet"@en;
  skos:definition "17. Did you receive and read the ANC booklet?";
  skos:inScheme <http://PharmAccess/MomCare/>;
  skos:topConceptOf <http://PharmAccess/MomCare/> .

MomCare:Inform_time_delivery_visit a skos:Concept;
  skos:prefLabel "Inform_time_delivery_visit"@en;
  skos:definition "18. Did the doctor/nurse inform you when to come to the hospital to deliver your baby? [Read out all options and select most appropriate]";
  skos:inScheme <http://PharmAccess/MomCare/>;
  skos:topConceptOf <http://PharmAccess/MomCare/> .

MomCare:Transport_mode_delivery a skos:Concept;
  skos:prefLabel "Transport_mode_delivery"@en;
  skos:definition "19. What mode of transport did you use to access the facility for delivery?";
  skos:inScheme <http://PharmAccess/MomCare/>;
  skos:topConceptOf <http://PharmAccess/MomCare/> .

MomCare:Facility_delivery_choice_reason a skos:Concept;
  skos:prefLabel "Facility_delivery_choice_reason"@en;
  skos:definition "20. Why did you choose to deliver in the hospital you delivered in";
  skos:inScheme <http://PharmAccess/MomCare/>;
  skos:topConceptOf <http://PharmAccess/MomCare/> .

MomCare:Facility_delivery_choice_reason_text a skos:Concept;
  skos:prefLabel "Facility_delivery_choice_reason_text"@en;
  skos:definition "Text 20. Why did you choose to deliver in the hospital you delivered in";
  skos:inScheme <http://PharmAccess/MomCare/>;
  skos:topConceptOf <http://PharmAccess/MomCare/> .

MomCare:Recommend_facility_delivery a skos:Concept;
  skos:prefLabel "Recommend_facility_delivery"@en;
  skos:definition "21.Would you recommend your friend or Neighbour to deliver at your same facility?";
  skos:inScheme <http://PharmAccess/MomCare/>;
  skos:topConceptOf <http://PharmAccess/MomCare/> .

MomCare:Recommend_facility_delivery_text a skos:Concept;
  skos:prefLabel "Recommend_facility_delivery_text"@en;
  skos:definition "Text 22. Why did you say that?";
  skos:inScheme <http://PharmAccess/MomCare/>;
  skos:topConceptOf <http://PharmAccess/MomCare/> .

MomCare:Delivery_rating a skos:Concept;
  skos:prefLabel "Delivery_rating"@en;
  skos:definition "23. Using any number from 1 to 5, where 1 is the worst experience possible and 5 is the best experience possible, what number would you use to rate your delivery experience";
  skos:inScheme <http://PharmAccess/MomCare/>;
  skos:topConceptOf <http://PharmAccess/MomCare/> .

MomCare:Delivery_danger_signs a skos:Concept;
  skos:prefLabel "Delivery_danger_signs"@en;
  skos:definition "24. After the delivery, did the doctor/nurse tell you about danger signs that should bring you back to hospital for a review? [You can give examples of signs such as Fever, foul smelling discharge, bleeding]",
    "24n. After the early end of pregnancy or delivery, did the doctor/nurse alert you of danger signs that should bring you back to hospital for a review? [You can give examples of signs such as Fever, foul smelling discharge, bleeding]";
  skos:inScheme <http://PharmAccess/MomCare/>;
  skos:topConceptOf <http://PharmAccess/MomCare/> .

MomCare:Information_enough a skos:Concept;
  skos:prefLabel "Information_enough"@en;
  skos:definition "25. Were you given enough information to help you decide about your care?";
  skos:inScheme <http://PharmAccess/MomCare/>;
  skos:topConceptOf <http://PharmAccess/MomCare/> .

MomCare:Support_delivery a skos:Concept;
  skos:prefLabel "Support_delivery"@en;
  skos:definition "26. Did you feel supported by the doctor/nurse at your facility during your Delivery?";
  skos:inScheme <http://PharmAccess/MomCare/>;
  skos:topConceptOf <http://PharmAccess/MomCare/> .

MomCare:Support_ANC_PNC a skos:Concept;
  skos:prefLabel "Support_ANC_PNC"@en;
  skos:definition "27. Did you feel supported by the doctor/nurse at your facility during your Antenatal & Postnatal Clinic?";
  skos:inScheme <http://PharmAccess/MomCare/>;
  skos:topConceptOf <http://PharmAccess/MomCare/> .

MomCare:Breastfeeding_information a skos:Concept;
  skos:prefLabel "Breastfeeding_information"@en;
  skos:definition "30. Did the doctor/nurse give you any information on breastfeeding? For example, did they demonstrate the technique or give you any tips to increase milk supply?";
  skos:inScheme <http://PharmAccess/MomCare/>;
  skos:topConceptOf <http://PharmAccess/MomCare/> .

MomCare:Breastfeeding_challenges_1 a skos:Concept;
  skos:prefLabel "Breastfeeding_challenges_1"@en;
  skos:definition "31. Did you have any challenges breastfeeding? : 1";
  skos:inScheme <http://PharmAccess/MomCare/>;
  skos:topConceptOf <http://PharmAccess/MomCare/> .

MomCare:Breastfeeding_challenges_text a skos:Concept;
  skos:prefLabel "Breastfeeding_challenges_text"@en;
  skos:definition "Text 31. Did you have any challenges breastfeeding?";
  skos:inScheme <http://PharmAccess/MomCare/>;
  skos:topConceptOf <http://PharmAccess/MomCare/> .

MomCare:Health_challenges_daily_1 a skos:Concept;
  skos:prefLabel "Health_challenges_daily_1"@en;
  skos:definition "32. Did you experience any of the following challenges with your health (that limited your daily activities)? please say Yes or No for everything I mention: : 1";
  skos:inScheme <http://PharmAccess/MomCare/>;
  skos:topConceptOf <http://PharmAccess/MomCare/> .

MomCare:Mental_experience_post_delivery_1 a skos:Concept;
  skos:prefLabel "Mental_experience_post_delivery_1"@en;
  skos:definition "33. In the first month after delivery did you experience any or more of the following - please say Yes or No for every option I mention: : 1";
  skos:inScheme <http://PharmAccess/MomCare/>;
  skos:topConceptOf <http://PharmAccess/MomCare/> .

MomCare:Counselling a skos:Concept;
  skos:prefLabel "Counselling"@en;
  skos:definition "34. Did you receive any form of counselling?";
  skos:inScheme <http://PharmAccess/MomCare/>;
  skos:topConceptOf <http://PharmAccess/MomCare/> .

MomCare:Experience_overall a skos:Concept;
  skos:prefLabel "Experience_overall"@en;
  skos:definition "35. Would you describe your overall experience of the MomCare program, beyond the delivery, as good, average, or poor?";
  skos:inScheme <http://PharmAccess/MomCare/>;
  skos:topConceptOf <http://PharmAccess/MomCare/> .

MomCare:Experience_overall_reason a skos:Concept;
  skos:prefLabel "Experience_overall_reason"@en;
  skos:definition "Text 36. Why have you given the MomCare program that overall rating?";
  skos:inScheme <http://PharmAccess/MomCare/>;
  skos:topConceptOf <http://PharmAccess/MomCare/> .

MomCare:tz-diagn a skos:Concept;
  skos:prefLabel "tz-diagn"@en;
  skos:inScheme <http://PharmAccess/MomCare/>;
  skos:topConceptOf <http://PharmAccess/MomCare/> .

MomCare:PATIENT_ID a skos:Concept;
  skos:prefLabel "PATIENT_ID"@en;
  skos:definition "Identifier for all those enrolled in the MomCare program.";
  skos:inScheme <http://PharmAccess/MomCare/>;
  skos:topConceptOf <http://PharmAccess/MomCare/> .

MomCare:DATE_OF_BIRTH a skos:Concept;
  skos:prefLabel "DATE_OF_BIRTH"@en;
  skos:definition "Date of birth of identified beneficiary.";
  skos:inScheme <http://PharmAccess/MomCare/>;
  skos:topConceptOf <http://PharmAccess/MomCare/> .

MomCare:AGE_AT_ENROLMENT a skos:Concept;
  skos:prefLabel "AGE_AT_ENROLMENT"@en;
  skos:definition "Age at enrolment derived from date of birth and enrolment date.";
  skos:inScheme <http://PharmAccess/MomCare/>;
  skos:topConceptOf <http://PharmAccess/MomCare/> .

MomCare:ENROLMENT_DATE a skos:Concept;
  skos:prefLabel "ENROLMENT_DATE"@en;
  skos:definition "Date of enrolment in MomCare program. This date is sometimes manually adjusted to allow beneficiaries to qualify for enrolment.";
  skos:inScheme <http://PharmAccess/MomCare/>;
  skos:topConceptOf <http://PharmAccess/MomCare/> .

MomCare:ENROLMENT_PROVIDER_ID a skos:Concept;
  skos:prefLabel "ENROLMENT_PROVIDER_ID"@en;
  skos:definition "Identifier of care provider linked to the MomCare program";
  skos:inScheme <http://PharmAccess/MomCare/>;
  skos:topConceptOf <http://PharmAccess/MomCare/> .

MomCare:ENROLMENT_PROVIDER_NAME a skos:Concept;
  skos:prefLabel "ENROLMENT_PROVIDER_NAME"@en;
  skos:definition "Name of care provider linked to the MomCare program.";
  skos:inScheme <http://PharmAccess/MomCare/>;
  skos:topConceptOf <http://PharmAccess/MomCare/> .

MomCare:ENROLMENT_PROVIDER_LEVEL a skos:Concept;
  skos:prefLabel "ENROLMENT_PROVIDER_LEVEL"@en;
  skos:definition "Level of care provider linked to the MomCare program.";
  skos:inScheme <http://PharmAccess/MomCare/>;
  skos:topConceptOf <http://PharmAccess/MomCare/> .

MomCare:ENROLMENT_REGION a skos:Concept;
  skos:prefLabel "ENROLMENT_REGION"@en;
  skos:definition "Region of enrolment in MomCare program.";
  skos:inScheme <http://PharmAccess/MomCare/>;
  skos:topConceptOf <http://PharmAccess/MomCare/> .

MomCare:VISIT_ID a skos:Concept;
  skos:prefLabel "VISIT_ID"@en;
  skos:definition "Unique identifier of visit for this beneficiary registered at MomCare facility.",
    "Unique identifier for visit for this beneficiary registered at MomCare facility.";
  skos:inScheme <http://PharmAccess/MomCare/>;
  skos:topConceptOf <http://PharmAccess/MomCare/> .

MomCare:VISIT_DATE a skos:Concept;
  skos:prefLabel "VISIT_DATE"@en;
  skos:definition "Date of visit registered at MomCare facility.";
  skos:inScheme <http://PharmAccess/MomCare/>;
  skos:topConceptOf <http://PharmAccess/MomCare/> .

MomCare:VISIT_NUMBER a skos:Concept;
  skos:prefLabel "VISIT_NUMBER"@en;
  skos:definition "Sum of visit counts for linked individual beneficiary.";
  skos:inScheme <http://PharmAccess/MomCare/>;
  skos:topConceptOf <http://PharmAccess/MomCare/> .

MomCare:VISIT_TYPE a skos:Concept;
  skos:prefLabel "VISIT_TYPE"@en;
  skos:definition "Visit category based on billed item categorization.", "Label based on categorization of linked billing items (codes).";
  skos:inScheme <http://PharmAccess/MomCare/>;
  skos:topConceptOf <http://PharmAccess/MomCare/> .

MomCare:VISIT_PROVIDER_ID a skos:Concept;
  skos:prefLabel "VISIT_PROVIDER_ID"@en;
  skos:definition "Identifier of care provider linked to the MomCare program", "Identifier of care provider linked to the MomCare program.";
  skos:inScheme <http://PharmAccess/MomCare/>;
  skos:topConceptOf <http://PharmAccess/MomCare/> .

MomCare:VISIT_PROVIDER_NAME a skos:Concept;
  skos:prefLabel "VISIT_PROVIDER_NAME"@en;
  skos:definition "Name of care provider linked to the MomCare program.";
  skos:inScheme <http://PharmAccess/MomCare/>;
  skos:topConceptOf <http://PharmAccess/MomCare/> .

MomCare:VISIT_PROVIDER_LEVEL a skos:Concept;
  skos:prefLabel "VISIT_PROVIDER_LEVEL"@en;
  skos:definition "Level of care provider linked to the MomCare program.";
  skos:inScheme <http://PharmAccess/MomCare/>;
  skos:topConceptOf <http://PharmAccess/MomCare/> .

MomCare:VISIT_PROVIDER_REGION a skos:Concept;
  skos:prefLabel "VISIT_PROVIDER_REGION"@en;
  skos:definition "Region of enrolment in MomCare program.";
  skos:inScheme <http://PharmAccess/MomCare/>;
  skos:topConceptOf <http://PharmAccess/MomCare/> .

MomCare:EVENT a skos:Concept;
  skos:prefLabel "EVENT"@en;
  skos:definition "Type of event (DIAGNOSIS/VISIT/ITEM).";
  skos:inScheme <http://PharmAccess/MomCare/>;
  skos:topConceptOf <http://PharmAccess/MomCare/> .

MomCare:EVENT_ID a skos:Concept;
  skos:prefLabel "EVENT_ID"@en;
  skos:definition "Unique identifier for event for this beneficiary registered at MomCare facility.";
  skos:inScheme <http://PharmAccess/MomCare/>;
  skos:topConceptOf <http://PharmAccess/MomCare/> .

MomCare:EVENT_DESCRIPTION a skos:Concept;
  skos:prefLabel "EVENT_DESCRIPTION"@en;
  skos:definition "Description of event.";
  skos:inScheme <http://PharmAccess/MomCare/>;
  skos:topConceptOf <http://PharmAccess/MomCare/> .

MomCare:DIAGN_DESCRIPTION a skos:Concept;
  skos:prefLabel "DIAGN_DESCRIPTION"@en;
  skos:definition "Diagnosis description based on ICD10 code.";
  skos:inScheme <http://PharmAccess/MomCare/>;
  skos:topConceptOf <http://PharmAccess/MomCare/> .

MomCare:DIAGN_CODE a skos:Concept;
  skos:prefLabel "DIAGN_CODE"@en;
  skos:definition "Diagnosis classified as ICD10 code.";
  skos:inScheme <http://PharmAccess/MomCare/>;
  skos:topConceptOf <http://PharmAccess/MomCare/> .

MomCare:EVENT_COSTS a skos:Concept;
  skos:prefLabel "EVENT_COSTS"@en;
  skos:definition "Sum of costs for event.";
  skos:inScheme <http://PharmAccess/MomCare/>;
  skos:topConceptOf <http://PharmAccess/MomCare/> .

MomCare:VISIT_DIAGN_NO a skos:Concept;
  skos:prefLabel "VISIT_DIAGN_NO"@en;
  skos:definition "Count of diagnosis for linked unique visit.";
  skos:inScheme <http://PharmAccess/MomCare/>;
  skos:topConceptOf <http://PharmAccess/MomCare/> .

MomCare:DIAGN_NO a skos:Concept;
  skos:prefLabel "DIAGN_NO"@en;
  skos:definition "Sum of diagnosis counts for linked individual beneficiary.";
  skos:inScheme <http://PharmAccess/MomCare/>;
  skos:topConceptOf <http://PharmAccess/MomCare/> .

MomCare:ke-diagn a skos:Concept;
  skos:prefLabel "ke-diagn"@en;
  skos:definition "This is a set of controlled terms for the Kenyan diagnosis data.";
  skos:inScheme <http://PharmAccess/MomCare/>;
  skos:topConceptOf <http://PharmAccess/MomCare/> .

MomCare:EVENT_TYPE a skos:Concept;
  skos:prefLabel "EVENT_TYPE"@en;
  skos:definition "Type of event (DIAGNOSIS/VISIT/ITEM).";
  skos:inScheme <http://PharmAccess/MomCare/>;
  skos:topConceptOf <http://PharmAccess/MomCare/> .

MomCare:TREATMENT_ID a skos:Concept;
  skos:prefLabel "TREATMENT_ID"@en;
  skos:definition "Unique identifier for treatment for this beneficiary registered at MomCare facility, processed by CareAnalytics.";
  skos:inScheme <http://PharmAccess/MomCare/>;
  skos:topConceptOf <http://PharmAccess/MomCare/> .

MomCare:REFERENCE a skos:Concept;
  skos:prefLabel "REFERENCE"@en;
  skos:definition "Code.";
  skos:inScheme <http://PharmAccess/MomCare/>;
  skos:topConceptOf <http://PharmAccess/MomCare/> .

MomCare:DATE_TREATMENT a skos:Concept;
  skos:prefLabel "DATE_TREATMENT"@en;
  skos:definition "Date of visit registered at MomCare facility.";
  skos:inScheme <http://PharmAccess/MomCare/>;
  skos:topConceptOf <http://PharmAccess/MomCare/> .

MomCare:PROVIDER_ID a skos:Concept;
  skos:prefLabel "PROVIDER_ID"@en;
  skos:definition "Identifier of care provider linked to the MomCare program", "Identifier of care provider linked to the MomCare program.";
  skos:inScheme <http://PharmAccess/MomCare/>;
  skos:topConceptOf <http://PharmAccess/MomCare/> .

MomCare:PROVIDER a skos:Concept;
  skos:prefLabel "PROVIDER"@en;
  skos:definition "Name of care provider linked to the MomCare program.";
  skos:inScheme <http://PharmAccess/MomCare/>;
  skos:topConceptOf <http://PharmAccess/MomCare/> .

MomCare:TREATMENT_STATUS a skos:Concept;
  skos:prefLabel "TREATMENT_STATUS"@en;
  skos:definition "Label based on closed or open treatment status.";
  skos:inScheme <http://PharmAccess/MomCare/>;
  skos:topConceptOf <http://PharmAccess/MomCare/> .

MomCare:PAYMENT_STATUS a skos:Concept;
  skos:prefLabel "PAYMENT_STATUS"@en;
  skos:definition "Label based on approved or rejected payment status.";
  skos:inScheme <http://PharmAccess/MomCare/>;
  skos:topConceptOf <http://PharmAccess/MomCare/> .

MomCare:TOTAL_COST a skos:Concept;
  skos:prefLabel "TOTAL_COST"@en;
  skos:definition "Sum of costs for event.";
  skos:inScheme <http://PharmAccess/MomCare/>;
  skos:topConceptOf <http://PharmAccess/MomCare/> .

MomCare:VISIT_DIAGNOSIS_ID a skos:Concept;
  skos:prefLabel "VISIT_DIAGNOSIS_ID"@en;
  skos:definition "Unique identifier for visit and diagnosis given.";
  skos:inScheme <http://PharmAccess/MomCare/>;
  skos:topConceptOf <http://PharmAccess/MomCare/> .

MomCare:DIAGNOSIS_ID a skos:Concept;
  skos:prefLabel "DIAGNOSIS_ID"@en;
  skos:definition "Unique identifier of diagnosis given.";
  skos:inScheme <http://PharmAccess/MomCare/>;
  skos:topConceptOf <http://PharmAccess/MomCare/> .

MomCare:DIAGN_LABEL a skos:Concept;
  skos:prefLabel "DIAGN_LABEL"@en;
  skos:definition "Diagnosis description based on ICD10 code.";
  skos:inScheme <http://PharmAccess/MomCare/>;
  skos:topConceptOf <http://PharmAccess/MomCare/> .

MomCare:DIAGN_CAT a skos:Concept;
  skos:prefLabel "DIAGN_CAT"@en;
  skos:definition "Diagnosis category based on ICD10 code generated for regression analysis Kenya (general and specific).";
  skos:inScheme <http://PharmAccess/MomCare/>;
  skos:topConceptOf <http://PharmAccess/MomCare/> .

MomCare:DIAG_gen a skos:Concept;
  skos:prefLabel "DIAG_gen"@en;
  skos:definition "Diagnosis category based on ICD10 code generated for regression analysis Kenya (general).";
  skos:inScheme <http://PharmAccess/MomCare/>;
  skos:topConceptOf <http://PharmAccess/MomCare/> .

MomCare:DIAGNOSIS a skos:Concept;
  skos:prefLabel "DIAGNOSIS"@en;
  skos:definition "Diagnosis category based on ICD10 code generated for regression analysis Kenya (specific).";
  skos:inScheme <http://PharmAccess/MomCare/>;
  skos:topConceptOf <http://PharmAccess/MomCare/> .

MomCare:DIAGNOSIS_CA a skos:Concept;
  skos:prefLabel "DIAGNOSIS_CA"@en;
  skos:definition "Diagnosis category based on ICD10 code generated by Care Analytics.";
  skos:inScheme <http://PharmAccess/MomCare/>;
  skos:topConceptOf <http://PharmAccess/MomCare/> .

MomCare:VISIT_NO a skos:Concept;
  skos:prefLabel "VISIT_NO"@en;
  skos:definition "Sum of visit counts for linked individual beneficiary.";
  skos:inScheme <http://PharmAccess/MomCare/>;
  skos:topConceptOf <http://PharmAccess/MomCare/> .

MomCare:ke-items a skos:Concept;
  skos:prefLabel "ke-items"@en;
  skos:definition "This is a set of controlled terms for the Kenyan billing items data.";
  skos:inScheme <http://PharmAccess/MomCare/>;
  skos:topConceptOf <http://PharmAccess/MomCare/> .

MomCare:CARE_ANALYTICS_ID a skos:Concept;
  skos:prefLabel "CARE_ANALYTICS_ID"@en;
  skos:definition "Identifier for those enrolled in the MomCare program and registered in Care Analytics (only Kenyan beneficiaries).";
  skos:inScheme <http://PharmAccess/MomCare/>;
  skos:topConceptOf <http://PharmAccess/MomCare/> .

MomCare:BENEFICIARY_ID_ORG a skos:Concept;
  skos:prefLabel "BENEFICIARY_ID_ORG"@en;
  skos:definition "Identifier of care provider linked to the MomCare program.";
  skos:inScheme <http://PharmAccess/MomCare/>;
  skos:topConceptOf <http://PharmAccess/MomCare/> .

MomCare:ITEM_ID a skos:Concept;
  skos:prefLabel "ITEM_ID"@en;
  skos:definition "Unique identifier of item billed.";
  skos:inScheme <http://PharmAccess/MomCare/>;
  skos:topConceptOf <http://PharmAccess/MomCare/> .

MomCare:ITEM_CODE a skos:Concept;
  skos:prefLabel "ITEM_CODE"@en;
  skos:definition "Label to signifiy type of item billed.";
  skos:inScheme <http://PharmAccess/MomCare/>;
  skos:topConceptOf <http://PharmAccess/MomCare/> .

MomCare:ITEM_NAME a skos:Concept;
  skos:prefLabel "ITEM_NAME"@en;
  skos:definition "Description of type of item billed.";
  skos:inScheme <http://PharmAccess/MomCare/>;
  skos:topConceptOf <http://PharmAccess/MomCare/> .

MomCare:tz-items a skos:Concept;
  skos:prefLabel "tz-items"@en;
  skos:definition "This is a set of controlled terms for the Tanzanian billing items data.";
  skos:inScheme <http://PharmAccess/MomCare/>;
  skos:topConceptOf <http://PharmAccess/MomCare/> .

MomCare:VISIT_ITEM_NO a skos:Concept;
  skos:prefLabel "VISIT_ITEM_NO"@en;
  skos:definition "Count of items for linked unique visit.";
  skos:inScheme <http://PharmAccess/MomCare/>;
  skos:topConceptOf <http://PharmAccess/MomCare/> .

MomCare:ITEM_NO a skos:Concept;
  skos:prefLabel "ITEM_NO"@en;
  skos:definition "Sum of items count for linked individual beneficiary.";
  skos:inScheme <http://PharmAccess/MomCare/>;
  skos:topConceptOf <http://PharmAccess/MomCare/> .

MomCare:safe_care a skos:Concept;
  skos:prefLabel "safe_care"@en;
  skos:definition "This is a set of controlled terms for the SafeCare quality assessment data.";
  skos:inScheme <http://PharmAccess/MomCare/>;
  skos:topConceptOf <http://PharmAccess/MomCare/> .

<http://PharmAccess/MomCare/#Assessment%20ID> a skos:Concept;
  skos:prefLabel "Assessment ID"@en;
  skos:definition "Unique identifier of SafeCare Assessment performed.";
  skos:inScheme <http://PharmAccess/MomCare/>;
  skos:topConceptOf <http://PharmAccess/MomCare/> .

<http://PharmAccess/MomCare/#Facility%20ID> a skos:Concept;
  skos:prefLabel "Facility ID"@en;
  skos:definition "Unique identifier for provider as registered by SafeCare.";
  skos:inScheme <http://PharmAccess/MomCare/>;
  skos:topConceptOf <http://PharmAccess/MomCare/> .

MomCare:Facility a skos:Concept;
  skos:prefLabel "Facility"@en;
  skos:definition "Name of care provider as registered by SafeCare.";
  skos:inScheme <http://PharmAccess/MomCare/>;
  skos:topConceptOf <http://PharmAccess/MomCare/> .

MomCare:District a skos:Concept;
  skos:prefLabel "District"@en;
  skos:definition "District location of care provider as registered by SafeCare.";
  skos:inScheme <http://PharmAccess/MomCare/>;
  skos:topConceptOf <http://PharmAccess/MomCare/> .

MomCare:Region a skos:Concept;
  skos:prefLabel "Region"@en;
  skos:definition "Region location of care provider as registered by SafeCare.";
  skos:inScheme <http://PharmAccess/MomCare/>;
  skos:topConceptOf <http://PharmAccess/MomCare/> .

<http://PharmAccess/MomCare/#Facility%20category> a skos:Concept;
  skos:prefLabel "Facility category"@en;
  skos:definition "Category of facility as registered by SafeCare.";
  skos:inScheme <http://PharmAccess/MomCare/>;
  skos:topConceptOf <http://PharmAccess/MomCare/> .

MomCare:Latitude a skos:Concept;
  skos:prefLabel "Latitude"@en;
  skos:definition "Latitude location of care provider as registered by SafeCare.";
  skos:inScheme <http://PharmAccess/MomCare/>;
  skos:topConceptOf <http://PharmAccess/MomCare/> .

MomCare:Longitude a skos:Concept;
  skos:prefLabel "Longitude"@en;
  skos:definition "Longitude location of care provider as registered by SafeCare.";
  skos:inScheme <http://PharmAccess/MomCare/>;
  skos:topConceptOf <http://PharmAccess/MomCare/> .

<http://PharmAccess/MomCare/#Approval%20date> a skos:Concept;
  skos:prefLabel "Approval date"@en;
  skos:definition "Date of approval as registered by SafeCare.";
  skos:inScheme <http://PharmAccess/MomCare/>;
  skos:topConceptOf <http://PharmAccess/MomCare/> .

<http://PharmAccess/MomCare/#Visit%20number> a skos:Concept;
  skos:prefLabel "Visit number"@en;
  skos:definition "Number of visit as registered by SafeCare.";
  skos:inScheme <http://PharmAccess/MomCare/>;
  skos:topConceptOf <http://PharmAccess/MomCare/> .

<http://PharmAccess/MomCare/#Type%20of%20ownership> a skos:Concept;
  skos:prefLabel "Type of ownership"@en;
  skos:definition "Type of ownership location of care provider as registered by SafeCare.";
  skos:inScheme <http://PharmAccess/MomCare/>;
  skos:topConceptOf <http://PharmAccess/MomCare/> .

MomCare:Location a skos:Concept;
  skos:prefLabel "Location"@en;
  skos:definition "Urban or rual categorization of care provider as registered by SafeCare.";
  skos:inScheme <http://PharmAccess/MomCare/>;
  skos:topConceptOf <http://PharmAccess/MomCare/> .

<http://PharmAccess/MomCare/#Assessment%20Tool> a skos:Concept;
  skos:prefLabel "Assessment Tool"@en;
  skos:definition "Tool of assessment as registered by SafeCare.";
  skos:inScheme <http://PharmAccess/MomCare/>;
  skos:topConceptOf <http://PharmAccess/MomCare/> .

MomCare:Version a skos:Concept;
  skos:prefLabel "Version"@en;
  skos:definition "Version of assessment tool as registered by SafeCare.";
  skos:inScheme <http://PharmAccess/MomCare/>;
  skos:topConceptOf <http://PharmAccess/MomCare/> .

<http://PharmAccess/MomCare/#Team%20leader> a skos:Concept;
  skos:prefLabel "Team leader"@en;
  skos:definition "Leader of team as registered by SafeCare.";
  skos:inScheme <http://PharmAccess/MomCare/>;
  skos:topConceptOf <http://PharmAccess/MomCare/> .

<http://PharmAccess/MomCare/#Team%20members> a skos:Concept;
  skos:prefLabel "Team members"@en;
  skos:definition "Members of team as registered by SafeCare.";
  skos:inScheme <http://PharmAccess/MomCare/>;
  skos:topConceptOf <http://PharmAccess/MomCare/> .

<http://PharmAccess/MomCare/#First%20reviewer> a skos:Concept;
  skos:prefLabel "First reviewer"@en;
  skos:definition "First reviewer of team as registered by SafeCare.";
  skos:inScheme <http://PharmAccess/MomCare/>;
  skos:topConceptOf <http://PharmAccess/MomCare/> .

<http://PharmAccess/MomCare/#SC%20Level%20calculated> a skos:Concept;
  skos:prefLabel "SC Level calculated"@en;
  skos:definition "SC Level calculated based on assessment of provider.";
  skos:inScheme <http://PharmAccess/MomCare/>;
  skos:topConceptOf <http://PharmAccess/MomCare/> .

<http://PharmAccess/MomCare/#SafeCare%20Score%20Rating%20(Basic)> a skos:Concept;
  skos:prefLabel "SafeCare Score Rating (Basic)"@en;
  skos:definition "SafeCare Score Rating (Basic) based on assesment of provider.";
  skos:inScheme <http://PharmAccess/MomCare/>;
  skos:topConceptOf <http://PharmAccess/MomCare/> .

<http://PharmAccess/MomCare/#SafeCare%20Score%20Advanced> a skos:Concept;
  skos:prefLabel "SafeCare Score Advanced"@en;
  skos:definition "SafeCare Score Advanced based on asssement of provider.";
  skos:inScheme <http://PharmAccess/MomCare/>;
  skos:topConceptOf <http://PharmAccess/MomCare/> .

<http://PharmAccess/MomCare/#SC%20Level%20awarded> a skos:Concept;
  skos:prefLabel "SC Level awarded"@en;
  skos:definition "SC level awarded based on SC score.";
  skos:inScheme <http://PharmAccess/MomCare/>;
  skos:topConceptOf <http://PharmAccess/MomCare/> .

MomCare:Organization a skos:Concept;
  skos:prefLabel "Organization"@en;
  skos:definition "Organization performing SafeCare assessment";
  skos:inScheme <http://PharmAccess/MomCare/>;
  skos:topConceptOf <http://PharmAccess/MomCare/> .

MomCare:Program a skos:Concept;
  skos:prefLabel "Program"@en;
  skos:definition "Business program providing funds for SafeCare assesment.";
  skos:inScheme <http://PharmAccess/MomCare/>;
  skos:topConceptOf <http://PharmAccess/MomCare/> .

<http://PharmAccess/MomCare/#SE1%20Score> a skos:Concept;
  skos:prefLabel "SE1 Score"@en;
  skos:definition "First SafeCare score.";
  skos:inScheme <http://PharmAccess/MomCare/>;
  skos:topConceptOf <http://PharmAccess/MomCare/> .

<http://PharmAccess/MomCare/#SE2%20Score> a skos:Concept;
  skos:prefLabel "SE2 Score"@en;
  skos:definition "Second SafeCare score.";
  skos:inScheme <http://PharmAccess/MomCare/>;
  skos:topConceptOf <http://PharmAccess/MomCare/> .

<http://PharmAccess/MomCare/#SE3%20Score> a skos:Concept;
  skos:prefLabel "SE3 Score"@en;
  skos:definition "Third SafeCare score.";
  skos:inScheme <http://PharmAccess/MomCare/>;
  skos:topConceptOf <http://PharmAccess/MomCare/> .

<http://PharmAccess/MomCare/#SE4%20Score> a skos:Concept;
  skos:prefLabel "SE4 Score"@en;
  skos:definition "Fourth SafeCare score.";
  skos:inScheme <http://PharmAccess/MomCare/>;
  skos:topConceptOf <http://PharmAccess/MomCare/> .

<http://PharmAccess/MomCare/#SE5%20Score> a skos:Concept;
  skos:prefLabel "SE5 Score"@en;
  skos:definition "Fifth SafeCare score.";
  skos:inScheme <http://PharmAccess/MomCare/>;
  skos:topConceptOf <http://PharmAccess/MomCare/> .

<http://PharmAccess/MomCare/#SE6%20Score> a skos:Concept;
  skos:prefLabel "SE6 Score"@en;
  skos:definition "Sixth SafeCare score.";
  skos:inScheme <http://PharmAccess/MomCare/>;
  skos:topConceptOf <http://PharmAccess/MomCare/> .

<http://PharmAccess/MomCare/#SE7%20Score> a skos:Concept;
  skos:prefLabel "SE7 Score"@en;
  skos:definition "Seventh SafeCare score.";
  skos:inScheme <http://PharmAccess/MomCare/>;
  skos:topConceptOf <http://PharmAccess/MomCare/> .

<http://PharmAccess/MomCare/#SE8%20Score> a skos:Concept;
  skos:prefLabel "SE8 Score"@en;
  skos:definition "Eight SafeCare score.";
  skos:inScheme <http://PharmAccess/MomCare/>;
  skos:topConceptOf <http://PharmAccess/MomCare/> .

<http://PharmAccess/MomCare/#SE9%20Score> a skos:Concept;
  skos:prefLabel "SE9 Score"@en;
  skos:definition "Ninth SafeCare score.";
  skos:inScheme <http://PharmAccess/MomCare/>;
  skos:topConceptOf <http://PharmAccess/MomCare/> .

<http://PharmAccess/MomCare/#SE10%20Score> a skos:Concept;
  skos:prefLabel "SE10 Score"@en;
  skos:definition "Tenth SafeCare score.";
  skos:inScheme <http://PharmAccess/MomCare/>;
  skos:topConceptOf <http://PharmAccess/MomCare/> .

<http://PharmAccess/MomCare/#SE11%20Score> a skos:Concept;
  skos:prefLabel "SE11 Score"@en;
  skos:definition "Eleventh SafeCare score.";
  skos:inScheme <http://PharmAccess/MomCare/>;
  skos:topConceptOf <http://PharmAccess/MomCare/> .

<http://PharmAccess/MomCare/#SE12%20Score> a skos:Concept;
  skos:prefLabel "SE12 Score"@en;
  skos:definition "Twelveth SafeCare score.";
  skos:inScheme <http://PharmAccess/MomCare/>;
  skos:topConceptOf <http://PharmAccess/MomCare/> .

<http://PharmAccess/MomCare/#SE13%20Score> a skos:Concept;
  skos:prefLabel "SE13 Score"@en;
  skos:definition "Thirteenth SafeCare score.";
  skos:inScheme <http://PharmAccess/MomCare/>;
  skos:topConceptOf <http://PharmAccess/MomCare/> .
